concurrency/handoverhand/Impl.i.dfy
@@ -1,0 +1,604 @@
+include "../framework/GhostLinearSequence.i.dfy"
+include "../framework/Mutex.s.dfy"
+include "ShardedHashTableTokens.i.dfy"
+include "ShardedHashTable.i.dfy"
+include "../../lib/Lang/LinearSequence.i.dfy"
+include "../../lib/Base/sequences.i.dfy"
+
+module Impl {
+  import opened NativeTypes
+  import opened Options
+  import opened Sequences
+  import opened GhostLinearMaybe
+  import opened GhostLinearSequence_s
+  import opened GhostLinearSequence_i
+  import opened Mutexes
+
+  import opened Limits
+  import opened KeyValueType
+  import MapIfc
+  // import SSM = HashTableStubSSM
+
+  import opened LinearSequence_i
+  import opened LinearSequence_s
+
+  import opened SSM = ShardedHashTable
+  // import TST = ShardedHashTableTokens 
+  // import T = TST.T
+  import PCM = TicketStubPCM(MapIfc, SSM)
+  import T = Tokens(PCM)
+  import TST = TicketStubToken(MapIfc, SSM) 
+
+  import opened GhostLoc
+
+  type Token = T.Token
+
+  linear datatype Cap = Cap(
+    remaining: nat,
+    glinear resource: Token)
+  {
+    predicate Inv(loc: Loc)
+    {
+      && remaining <= Capacity()
+      && resource == T.Token(loc, unit()
+        .(insert_capacity := remaining))
+    }
+  }
+
+  linear datatype Row = Row(
+    entry: Entry,
+    glinear resource: Token)
+
+  predicate RowInv(loc: Loc, index: nat, row: Row)
+  {
+    && 0 <= index as nat < FixedSize()
+    && row.resource == T.Token(loc, oneRowResource(index as nat, Info(row.entry, Free), 0))
+  }
+
+  type RowMutex = Mutex<Row>
+
+  type RowMutexTable = lseq<RowMutex>
+  
+  predicate RowMutexTablePartialInv(row_mutexes: RowMutexTable, loc: Loc, index: nat)
+    requires index <= |row_mutexes| == FixedSize()
+  {
+    && (forall i | 0 <= i < index ::
+      (i in row_mutexes) && (row_mutexes[i].inv == ((row: Row) => RowInv(loc, i, row))))
+    && (forall i | index <= i < |row_mutexes| ::
+      (i !in row_mutexes))
+  }
+
+  predicate RowMutexTableInv(row_mutexes: RowMutexTable, loc: Loc)
+    requires |row_mutexes| == FixedSize()
+  {
+    RowMutexTablePartialInv(row_mutexes, loc, |row_mutexes|)
+  }
+
+  linear datatype IVariables = IVariables(
+    linear row_mutexes: RowMutexTable,
+    linear cap_mutex: Mutex<Cap>)
+  {
+    predicate Inv(loc: Loc)
+    {
+      && |row_mutexes| == FixedSize()
+      && RowMutexTableInv(row_mutexes, loc)
+      && (cap_mutex.inv == ((cap: Cap) => cap.Inv(loc)))
+    }
+  }
+
+  datatype Splitted = Splitted(expected:SSM.M, ri:SSM.M)
+
+  function {:opaque} InitResoucePartial(i: nat): SSM.M
+    requires i <= FixedSize()
+  {
+    var table := seq(FixedSize(), j => if j >= i then Some(Info(Empty, Free)) else None);
+    SSM.M(table, Capacity(), multiset{}, multiset{})
+  }
+
+  function Split(r:SSM.M, i:nat) : (splt:Splitted)
+    requires i < FixedSize()
+    requires r == InitResoucePartial(i)
+    ensures SSM.dot(splt.expected, splt.ri) == r
+  {
+    var expected := InitResoucePartial(i+1);
+    var ri := oneRowResource(i as nat, Info(Empty, Free), 0);
+    reveal InitResoucePartial();
+    Splitted(expected, ri)
+  }
+
+  method init(glinear in_token: Token)
+  returns (glinear token: Token, linear iv: IVariables)
+    requires in_token.val == SSM.Init()
+    // ensures Inv(v)
+    ensures token.val == SSM.unit()
+  {
+    var loc := in_token.loc;
+
+    token := in_token;
+    linear var row_mutexes :RowMutexTable := lseq_alloc(FixedSizeImpl() as uint64);
+
+    var i:uint32 := 0;
+
+    assert token.val == InitResoucePartial(0) by {
+      reveal InitResoucePartial();
+    }
+
+    while i < FixedSizeImpl()
+      invariant token.loc == loc
+      invariant i as int <= |row_mutexes| == FixedSize()
+      invariant token.val == InitResoucePartial(i as nat)
+      invariant RowMutexTablePartialInv(row_mutexes, loc, i as nat)
+    {
+      ghost var splitted := Split(token.val, i as int);
+      glinear var mutex_token := T.inout_split(inout token, splitted.expected, splitted.ri);
+      linear var m := new_mutex<Row>(Row(Empty, mutex_token),
+        (row: Row) => RowInv(loc, i as nat, row));
+  
+      lseq_give_inout(inout row_mutexes, i as uint64, m);
+
+      i := i + 1;
+    }
+
+    assert token.val == SSM.unit().(insert_capacity := Capacity()) by {
+      reveal InitResoucePartial();
+    }
+
+    glinear var mutex_token := T.inout_split(inout token, SSM.unit(), SSM.unit().(insert_capacity := Capacity()));
+
+    linear var cap_mutex := new_mutex<Cap>(Cap(CapacityImpl() as nat, mutex_token),
+      (cap: Cap) => cap.Inv(loc));
+    
+    iv := IVariables.IVariables(row_mutexes, cap_mutex);
+  }
+
+  predicate method shouldHashGoBefore(search_h: uint32, slot_h: uint32, slot_idx: uint32) 
+    ensures shouldHashGoBefore(search_h, slot_h, slot_idx) 
+      == ShouldHashGoBefore(search_h as int, slot_h as int, slot_idx as int)
+  {
+    || search_h < slot_h <= slot_idx // normal case
+    || slot_h <= slot_idx < search_h // search_h wraps around the end of array
+    || slot_idx < search_h < slot_h// search_h, slot_h wrap around the end of array
+  }
+
+  function method getNextIndex(slot_idx: uint32) : uint32
+    requires slot_idx < FixedSizeImpl()
+  {
+    if slot_idx == FixedSizeImpl() - 1 then 0 else slot_idx + 1
+  }
+
+  method acquireRow(shared iv: IVariables, index: uint32, glinear in_token: Token)
+  returns (entry: Entry, glinear handle: MutexHandle<Row>, glinear out_token: Token)
+    requires iv.Inv(in_token.loc)
+    requires index < FixedSizeImpl();
+    ensures handle.m == iv.row_mutexes[index as nat];
+    ensures out_token.loc == in_token.loc;
+    ensures out_token.val == dot(in_token.val, oneRowResource(index as nat, Info(entry, Free), 0))
+  {
+    linear var row; 
+    row, handle := lseq_peek(iv.row_mutexes, index as uint64).acquire();
+    linear var Row(out_entry, row_token) := row;
+
+    entry := out_entry;
+
+    out_token := T.join(in_token, row_token);
+  }
+
+  method releaseRow(
+    shared iv: IVariables,
+    index: uint32,
+    entry: Entry,
+    glinear handle: MutexHandle<Row>,
+    glinear in_token: Token)
+  returns (glinear out_token: Token)
+    requires iv.Inv(in_token.loc);
+    requires index < FixedSizeImpl();
+    requires handle.m == iv.row_mutexes[index as nat];
+    requires in_token.val.M?;
+    requires in_token.val.table[index as nat] == Some(Info(entry, Free));
+    ensures out_token.loc == in_token.loc;
+    ensures out_token.val == in_token.val.(table := in_token.val.table[index := None]);
+  {
+    glinear var mutex_token;
+    ghost var left := in_token.val.(table := in_token.val.table[index := None]);
+    ghost var right := oneRowResource(index as nat, Info(entry, Free), 0);
+
+    out_token, mutex_token := T.split(in_token, left, right);
+
+    lseq_peek(iv.row_mutexes, index as uint64).release(Row(entry, mutex_token), handle);
+  }
+
+  linear method acquireCapacity(shared iv: IVariables, glinear in_token: Token)
+  returns (glinear out_token: Token)
+    decreases *
+    requires iv.Inv(in_token.loc)
+    requires in_token.val.M?;
+
+    ensures out_token ==
+      in_token.(val := in_token.val.(insert_capacity := in_token.val.insert_capacity + 1))
+  {
+    ghost var old_token := in_token;
+    ghost var old_cap := in_token.val.insert_capacity;
+    out_token := in_token;
+    var continue := true;
+
+    while continue
+      invariant iv.Inv(old_token.loc)
+      invariant continue ==> out_token == old_token
+      invariant !continue ==> out_token == old_token.(val := old_token.val.(insert_capacity := old_cap + 1))
+      decreases *
+    {
+      linear var cap; glinear var handle: MutexHandle<Cap>;
+      cap, handle := iv.cap_mutex.acquire();
+
+      linear var Cap(count, cap_token) := cap;
+
+      if count >= 1 {
+        count := count - 1;
+        ghost var left := SSM.unit().(insert_capacity := count);
+        ghost var right := SSM.unit().(insert_capacity := 1);
+        assert SSM.dot(left, right) == cap_token.val; 
+        glinear var temp_token := T.inout_split(inout cap_token, left, right);
+        T.inout_join(inout out_token, temp_token);
+        continue := false;
+      }
+
+      iv.cap_mutex.release(Cap(count, cap_token), handle);
+    }
+  }
+
+  linear method releaseCapacity(shared iv: IVariables, glinear in_token: Token)
+  returns (glinear out_token: Token)
+    requires iv.Inv(in_token.loc)
+    requires in_token.val.M?;
+    requires in_token.val.insert_capacity == 1
+
+    ensures out_token ==
+      in_token.(val := in_token.val.(insert_capacity := in_token.val.insert_capacity - 1))
+  {
+    linear var cap; glinear var handle: MutexHandle<Cap>;
+    cap, handle := iv.cap_mutex.acquire();
+
+    linear var Cap(count, cap_token) := cap;
+
+    count := count + 1;
+    ghost var left := in_token.val.(insert_capacity := 0);
+    ghost var right := SSM.unit().(insert_capacity := 1);
+    assert SSM.dot(left, right) == in_token.val; 
+    out_token := in_token;
+    glinear var temp_token := T.inout_split(inout out_token, left, right);
+    T.inout_join(inout cap_token, temp_token);
+
+    iv.cap_mutex.release(Cap(count, cap_token), handle);
+  }
+
+  method doQuery(shared iv: IVariables, input: MapIfc.Input, rid: nat, glinear in_token: Token)
+  returns (output: MapIfc.Output, glinear out_token: Token)
+    requires iv.Inv(in_token.loc)
+    requires input.QueryInput?
+    requires in_token.val == SSM.Ticket(rid, input)
+    ensures out_token.val == SSM.Stub(rid, output)
+    decreases *
+  {
+    ghost var loc := in_token.loc;
+    var query_ticket := SSM.Request(rid, input);
+    var key, hash_idx := input.key, hash(input.key);
+    var slot_idx := hash_idx;
+
+    var entry; glinear var handle;
+    entry, handle, out_token := acquireRow(iv, hash_idx, in_token);
+
+    var step := ProcessQueryTicketStep(query_ticket);
+    var expected := SSM.GetTransition(out_token.val, step);
+    out_token := TST.transition_1_1(out_token, expected);
+
+    while true 
+      invariant iv.Inv(loc);
+      invariant 0 <= slot_idx < FixedSizeImpl();
+      invariant out_token.loc == loc;
+      invariant out_token.val == oneRowResource(slot_idx as nat, Info(entry, Querying(rid, key)), 0);
+      invariant handle.m == iv.row_mutexes[slot_idx as nat];
+      decreases *
+    {
+      var next_slot_idx := getNextIndex(slot_idx);
+
+      match entry {
+        case Empty => {
+          output := MapIfc.QueryOutput(NotFound);
+          step := QueryNotFoundStep(slot_idx as nat);
+        }
+        case Full(KV(entry_key, value)) => {
+          if entry_key == key {
+            step := QueryDoneStep(slot_idx as nat);
+            output := MapIfc.QueryOutput(Found(value));
+          } else {
+            var should_go_before := shouldHashGoBefore(hash_idx, hash(entry_key), slot_idx);
+            if !should_go_before {
+              step := QuerySkipStep(slot_idx as nat);
+            } else {
+              output := MapIfc.QueryOutput(NotFound);
+              step := QueryNotFoundStep(slot_idx as nat);
+            }
+          }
+        }
+      }
+
+      if !step.QuerySkipStep? {
+        // this test is required for termination, but is not enforced by verification
+        // because we are using decreases *
+        break;
+      }
+    
+      var next_entry; glinear var next_handle;
+      next_entry, next_handle, out_token := acquireRow(iv, next_slot_idx, out_token);
+
+      expected := SSM.GetTransition(out_token.val, step);
+      out_token := TST.transition_1_1(out_token, expected);
+
+      out_token := releaseRow(iv, slot_idx, entry, handle, out_token);
+
+      slot_idx, entry := next_slot_idx, next_entry;
+      handle := next_handle;
+    }
+    
+    assert step.QueryNotFoundStep? || step.QueryDoneStep?;
+    expected := SSM.GetTransition(out_token.val, step);
+    out_token := TST.transition_1_1(out_token, expected);
+    out_token := releaseRow(iv, slot_idx, entry, handle, out_token);
+  }
+
+  method doInsert(shared iv: IVariables, input: MapIfc.Input, rid: nat, thread_id: uint32, glinear in_token: Token)
+  returns (output: MapIfc.Output, glinear out_token: Token)
+    requires iv.Inv(in_token.loc)
+    requires input.InsertInput?
+    requires in_token.val == SSM.Ticket(rid, input)
+    ensures out_token.val == SSM.Stub(rid, output)
+    decreases *
+  {
+    ghost var loc := in_token.loc;
+
+    var key, inital_key := input.key, input.key;
+    var kv := KV(key, input.value);
+    output := MapIfc.InsertOutput(true);
+
+    var hash_idx := hash(key);
+    var slot_idx := hash_idx;
+
+    out_token := acquireCapacity(iv, in_token);
+
+    var entry; glinear var handle;
+    entry, handle, out_token := acquireRow(iv, slot_idx, out_token);
+
+    var step := ProcessInsertTicketStep(SSM.Request(rid, input));
+    var expected := SSM.GetTransition(out_token.val, step);
+    out_token := TST.transition_1_1(out_token, expected);
+
+    while true 
+      invariant iv.Inv(loc)
+      invariant 0 <= slot_idx < FixedSizeImpl()
+      invariant out_token.loc == loc;
+      invariant out_token.val == oneRowResource(slot_idx as nat, Info(entry, Inserting(rid, kv, inital_key)), 0)
+      invariant kv.key == key
+      invariant hash_idx == hash(key)
+      invariant handle.m == iv.row_mutexes[slot_idx as nat];
+      decreases *
+    {
+      var next_slot_idx := getNextIndex(slot_idx);
+      var new_kv;
+
+      match entry {
+        case Empty => {
+          step := InsertDoneStep(slot_idx as nat);
+        }
+        case Full(KV(entry_key, value)) => {
+          new_kv := KV(entry_key, value);
+          if entry_key == key {
+            step := InsertUpdateStep(slot_idx as nat);
+          } else {
+            var should_go_before := shouldHashGoBefore(hash_idx, hash(entry_key), slot_idx);
+            if !should_go_before {
+              step := InsertSkipStep(slot_idx as nat);
+            } else {
+              step := InsertSwapStep(slot_idx as nat);
+            }
+          }
+        }
+      }
+
+      if step.InsertDoneStep? || step.InsertUpdateStep? {
+        break;
+      }
+
+      glinear var next_handle; var next_entry;
+      next_entry, next_handle, out_token := acquireRow(iv, next_slot_idx, out_token);
+
+      if step.InsertSwapStep? {
+        entry := Full(kv);
+        kv := new_kv;
+        key := new_kv.key;
+      }
+  
+      expected := SSM.GetTransition(out_token.val, step);
+      out_token := TST.transition_1_1(out_token, expected);
+      out_token := releaseRow(iv, slot_idx, entry, handle, out_token);
+
+      slot_idx, entry, hash_idx := next_slot_idx, next_entry, hash(key);
+      handle := next_handle;
+    }
+
+    // assert step.InsertDoneStep? || step.InsertUpdateStep?;
+    expected := SSM.GetTransition(out_token.val, step);
+    out_token := TST.transition_1_1(out_token, expected);
+
+    out_token := releaseRow(iv, slot_idx, Full(kv), handle, out_token);
+
+    if step.InsertUpdateStep? {
+      out_token := releaseCapacity(iv, out_token);
+      assert out_token.val.insert_capacity == 0;
+    }
+  }
+
+  method doRemoveFound(shared iv: IVariables, rid: nat, 
+    slot_idx: uint32,
+    hash_idx: uint32,
+    inital_key: Key,
+    entry: SSM.Entry,
+    glinear handle: MutexHandle<Row>,
+    glinear in_token: Token)
+  
+    returns (output: MapIfc.Output, glinear out_token: Token)
+    decreases *
+    requires iv.Inv(in_token.loc)
+    requires 0 <= slot_idx < FixedSizeImpl()
+    requires 0 <= hash_idx < FixedSizeImpl()
+    requires in_token.val == oneRowResource(slot_idx as nat, Info(entry, Removing(rid, inital_key)), 0);
+    requires entry.Full? && entry.kv.key == inital_key
+    requires hash(inital_key) == hash_idx
+    requires handle.m == iv.row_mutexes[slot_idx as nat]
+    ensures out_token.val == SSM.Stub(rid, output)
+  {
+    ghost var loc := in_token.loc;
+    var found_value := entry.kv.val;
+
+    var slot_idx := slot_idx;
+    var next_slot_idx := getNextIndex(slot_idx);
+
+    glinear var handle := handle;
+    glinear var next_handle; var next_entry;
+    out_token := in_token;
+    next_entry, next_handle, out_token := acquireRow(iv, next_slot_idx, out_token);
+
+    var step := RemoveFoundItStep(slot_idx as nat);
+
+    var expected := SSM.GetTransition(out_token.val, step);
+    out_token := TST.transition_1_1(out_token, expected);
+
+    while true
+      invariant iv.Inv(loc)
+      invariant 0 <= slot_idx < FixedSizeImpl()
+      invariant out_token.loc == loc
+      invariant out_token.val == twoRowsResource(
+        slot_idx as nat, Info(Empty, RemoveTidying(rid, inital_key, found_value)),
+        NextPos(slot_idx as nat), Info(next_entry, Free),
+        0)
+      invariant handle.m == iv.row_mutexes[slot_idx as nat]
+      invariant next_handle.m == iv.row_mutexes[NextPos(slot_idx as nat)]
+      decreases *
+    {
+      next_slot_idx := getNextIndex(slot_idx);
+
+      if next_entry.Empty? || (next_entry.Full? && hash(next_entry.kv.key) == next_slot_idx) {
+        assert DoneTidying(out_token.val, slot_idx as nat);
+        break;
+      }
+
+      expected := SSM.GetTransition(out_token.val, RemoveTidyStep(slot_idx as nat));
+      out_token := TST.transition_1_1(out_token, expected);
+      out_token := releaseRow(iv, slot_idx, next_entry, handle, out_token);
+
+      slot_idx := next_slot_idx;
+      next_slot_idx := getNextIndex(slot_idx);
+      handle := next_handle;
+
+      next_entry, next_handle, out_token := acquireRow(iv, next_slot_idx, out_token);
+    }
+    assert DoneTidying(out_token.val, slot_idx as nat);
+
+    next_slot_idx := getNextIndex(slot_idx);
+    output := MapIfc.RemoveOutput(true);
+
+    step := RemoveDoneStep(slot_idx as nat);
+    expected := SSM.GetTransition(out_token.val, step);
+    out_token := TST.transition_1_1(out_token, expected);
+
+    out_token := releaseRow(iv, slot_idx, Empty, handle, out_token);
+    out_token := releaseRow(iv, next_slot_idx, next_entry, next_handle, out_token);
+
+    out_token := releaseCapacity(iv, out_token);
+    assert out_token.val.insert_capacity == 0;
+  }
+
+  method doRemove(shared iv: IVariables, input: MapIfc.Input, rid: nat, thread_id: uint32, glinear in_token: Token)
+    returns (output: MapIfc.Output, glinear out_token: Token)
+    decreases *
+
+    requires iv.Inv(in_token.loc)
+    requires input.RemoveInput?
+    requires in_token.val == SSM.Ticket(rid, input)
+    ensures out_token.val == SSM.Stub(rid, output)
+  {
+    ghost var loc := in_token.loc;
+
+    var query_ticket := SSM.Request(rid, input);
+    var key := input.key;
+    var hash_idx := hash(key);
+    var slot_idx := hash_idx;
+
+    var entry; glinear var handle;
+    entry, handle, out_token := acquireRow(iv, slot_idx, in_token);
+
+    var step : Step := ProcessRemoveTicketStep(query_ticket);
+    // r := easy_transform_step(r, step);
+    var expected := SSM.GetTransition(out_token.val, step);
+    out_token := TST.transition_1_1(out_token, expected);
+
+    while true 
+      invariant iv.Inv(loc)
+      invariant 0 <= slot_idx < FixedSizeImpl()
+      invariant out_token.loc == loc
+      invariant out_token.val == oneRowResource(slot_idx as nat, Info(entry, Removing(rid, key)), 0)
+      invariant step.RemoveNotFoundStep? ==> 
+        (entry.Full? && shouldHashGoBefore(hash_idx, hash(entry.kv.key), slot_idx))
+      invariant step.RemoveTidyStep? ==> (
+        && TidyEnable(out_token.val, slot_idx as nat)
+        && KnowRowIsFree(out_token.val, NextPos(slot_idx as nat)))
+      invariant handle.m == iv.row_mutexes[slot_idx as nat]
+      decreases *
+    {
+      var next_slot_idx := getNextIndex(slot_idx);
+
+      match entry {
+        case Empty => {
+          step := RemoveNotFoundStep(slot_idx as nat);
+        }
+        case Full(KV(entry_key, value)) => {
+          if entry_key == key {
+            step := RemoveFoundItStep(slot_idx as nat);
+          } else {
+            var should_go_before := shouldHashGoBefore(hash_idx, hash(entry_key), slot_idx);
+
+            if !should_go_before {
+              step := RemoveSkipStep(slot_idx as nat);
+            } else {
+              step := RemoveNotFoundStep(slot_idx as nat);
+            }
+          }
+        }
+      }
+
+      if step.RemoveNotFoundStep? || step.RemoveFoundItStep? {
+        break;
+      }
+
+      glinear var next_handle; var next_entry;
+      next_entry, next_handle, out_token := acquireRow(iv, next_slot_idx, out_token);
+
+      expected := SSM.GetTransition(out_token.val, step);
+      out_token := TST.transition_1_1(out_token, expected);
+
+      out_token := releaseRow(iv, slot_idx, entry, handle, out_token);
+
+      slot_idx, entry := next_slot_idx, next_entry;
+      handle := next_handle;
+    }
+
+    if step.RemoveNotFoundStep? {
+      output := MapIfc.RemoveOutput(false);
+
+      expected := SSM.GetTransition(out_token.val, step);
+      out_token := TST.transition_1_1(out_token, expected);
+      out_token := releaseRow(iv, slot_idx, entry, handle, out_token);
+    } else {
+      output, out_token := doRemoveFound(iv, rid, slot_idx, hash_idx, key, entry, handle, out_token);
+    }
+  }
+}
